Weidenbach_Book/IsaSAT_Restart_LLVM.thy
@@ -1,0 +1,249 @@
+theory IsaSAT_Restart_LLVM
+  imports IsaSAT_Restart IsaSAT_Restart_Heuristics_LLVM IsaSAT_CDCL_LLVM
+begin
+
+sepref_register length_avdom
+
+sepref_register clause_is_learned_heur
+
+(*TODO Move: replace other verision*)
+lemma length_avdom_alt_def:
+  \<open>length_avdom = (\<lambda>(M', N', D', j, W', vm, \<phi>, clvls, cach, lbd, outl, stats, heur, vdom, avdom, lcount). length avdom)\<close>
+  by (intro ext) (auto simp: length_avdom_def)
+
+lemma get_the_propagation_reason_heur_alt_def:
+  \<open>get_the_propagation_reason_heur = (\<lambda>(M', N', D', j, W', vm, \<phi>, clvls, cach, lbd, outl, stats, heur, vdom, lcount) L .
+    get_the_propagation_reason_pol M' L)\<close>
+  by (intro ext) (auto simp: get_the_propagation_reason_heur_def)
+
+(*END Move*)
+
+sepref_def length_avdom_fast_code
+  is \<open>RETURN o length_avdom\<close>
+  :: \<open>isasat_bounded_assn\<^sup>k \<rightarrow>\<^sub>a sint64_nat_assn\<close>
+  unfolding length_avdom_alt_def access_vdom_at_pre_def isasat_bounded_assn_def
+  supply [[goals_limit = 1]]
+  by sepref
+
+sepref_register get_the_propagation_reason_heur
+
+sepref_def get_the_propagation_reason_heur_fast_code
+  is \<open>uncurry get_the_propagation_reason_heur\<close>
+  :: \<open>isasat_bounded_assn\<^sup>k *\<^sub>a unat_lit_assn\<^sup>k \<rightarrow>\<^sub>a snat_option_assn' TYPE(64)\<close>
+  unfolding get_the_propagation_reason_heur_alt_def access_vdom_at_pre_def
+     isasat_bounded_assn_def
+  supply [[goals_limit = 1]]
+  by sepref
+
+(*TODO Move: rplace*)
+
+lemma clause_is_learned_heur_alt_def:
+  \<open>clause_is_learned_heur = (\<lambda>(M', N', D', j, W', vm, \<phi>, clvls, cach, lbd, outl, stats, heur,
+    vdom, lcount) C . arena_status N' C = LEARNED)\<close>
+  by (intro ext) (auto simp: clause_is_learned_heur_def)
+(*ENED Move*)
+
+sepref_def clause_is_learned_heur_code2
+  is \<open>uncurry (RETURN oo clause_is_learned_heur)\<close>
+  :: \<open>[\<lambda>(S, C). arena_is_valid_clause_vdom (get_clauses_wl_heur S) C]\<^sub>a
+      isasat_bounded_assn\<^sup>k *\<^sub>a sint64_nat_assn\<^sup>k \<rightarrow> bool1_assn\<close>
+  supply [[goals_limit = 1]]
+  unfolding clause_is_learned_heur_alt_def isasat_bounded_assn_def
+  by sepref
+
+sepref_register clause_lbd_heur
+
+
+lemma clause_lbd_heur_alt_def:
+  \<open>clause_lbd_heur = (\<lambda>(M', N', D', j, W', vm, \<phi>, clvls, cach, lbd, outl, stats, heur, vdom, lcount) C.
+     arena_lbd N' C)\<close>
+  by (intro ext) (auto simp: clause_lbd_heur_def)
+
+sepref_def clause_lbd_heur_code2
+  is \<open>uncurry (RETURN oo clause_lbd_heur)\<close>
+  :: \<open>[\<lambda>(S, C). get_clause_LBD_pre (get_clauses_wl_heur S) C]\<^sub>a
+       isasat_bounded_assn\<^sup>k *\<^sub>a sint64_nat_assn\<^sup>k \<rightarrow> uint32_nat_assn\<close>
+  unfolding isasat_bounded_assn_def clause_lbd_heur_alt_def
+  supply [[goals_limit = 1]]
+  by sepref
+
+sepref_register mark_garbage_heur
+
+
+sepref_def mark_garbage_heur_code2
+  is \<open>uncurry2 (RETURN ooo mark_garbage_heur)\<close>
+  :: \<open>[\<lambda>((C, i), S). mark_garbage_pre (get_clauses_wl_heur S, C) \<and> i < length_avdom S \<and>
+         get_learned_count S \<ge> 1]\<^sub>a
+       sint64_nat_assn\<^sup>k *\<^sub>a sint64_nat_assn\<^sup>k *\<^sub>a isasat_bounded_assn\<^sup>d \<rightarrow> isasat_bounded_assn\<close>
+  supply [[goals_limit = 1]]
+  unfolding mark_garbage_heur_def isasat_bounded_assn_def delete_index_and_swap_alt_def
+    length_avdom_def fold_tuple_optimizations
+  apply (annot_unat_const "TYPE(64)")
+  by sepref
+
+sepref_register delete_index_vdom_heur
+
+
+sepref_def delete_index_vdom_heur_fast_code2
+  is \<open>uncurry (RETURN oo delete_index_vdom_heur)\<close>
+  :: \<open>[\<lambda>(i, S). i < length_avdom S]\<^sub>a
+        sint64_nat_assn\<^sup>k *\<^sub>a isasat_bounded_assn\<^sup>d \<rightarrow> isasat_bounded_assn\<close>
+  supply [[goals_limit = 1]]
+  unfolding delete_index_vdom_heur_def isasat_bounded_assn_def delete_index_and_swap_alt_def
+    length_avdom_def fold_tuple_optimizations
+  by sepref
+
+sepref_register access_length_heur
+
+sepref_def access_length_heur_fast_code2
+  is \<open>uncurry (RETURN oo access_length_heur)\<close>
+  :: \<open>[\<lambda>(S, C). arena_is_valid_clause_idx (get_clauses_wl_heur S) C]\<^sub>a
+       isasat_bounded_assn\<^sup>k *\<^sub>a sint64_nat_assn\<^sup>k \<rightarrow> sint64_nat_assn\<close>
+  supply [[goals_limit = 1]]
+  unfolding access_length_heur_alt_def isasat_bounded_assn_def fold_tuple_optimizations
+  by sepref
+
+sepref_register marked_as_used_st
+
+sepref_def marked_as_used_st_fast_code
+  is \<open>uncurry (RETURN oo marked_as_used_st)\<close>
+  :: \<open>[\<lambda>(S, C). marked_as_used_pre (get_clauses_wl_heur S) C]\<^sub>a
+       isasat_bounded_assn\<^sup>k *\<^sub>a sint64_nat_assn\<^sup>k \<rightarrow> bool1_assn\<close>
+  supply [[goals_limit = 1]]
+  unfolding marked_as_used_st_alt_def isasat_bounded_assn_def fold_tuple_optimizations
+  by sepref
+
+lemma arena_act_pre_mark_used:
+  \<open>arena_act_pre arena C \<Longrightarrow>
+  arena_act_pre (mark_unused arena C) C\<close>
+  unfolding arena_act_pre_def arena_is_valid_clause_idx_def
+  apply clarify
+  apply (rule_tac x=N in exI)
+  apply (rule_tac x=vdom in exI)
+  by (auto simp: arena_act_pre_def
+    simp: valid_arena_mark_unused)
+
+
+sepref_register mark_unused_st_heur
+sepref_def mark_unused_st_fast_code
+  is \<open>uncurry (RETURN oo mark_unused_st_heur)\<close>
+  :: \<open>[\<lambda>(C, S). arena_act_pre (get_clauses_wl_heur S) C]\<^sub>a
+        sint64_nat_assn\<^sup>k *\<^sub>a isasat_bounded_assn\<^sup>d \<rightarrow> isasat_bounded_assn\<close>
+  unfolding mark_unused_st_heur_def isasat_bounded_assn_def
+    arena_act_pre_mark_used[intro!]
+  supply [[goals_limit = 1]]
+  by sepref
+
+sepref_register mark_clauses_as_unused_wl_D_heur
+
+declare clause_not_marked_to_delete_heur_fast_code.refine[sepref_fr_rules]
+
+sepref_def mark_clauses_as_unused_wl_D_heur_fast_code
+  is \<open>uncurry mark_clauses_as_unused_wl_D_heur\<close>
+  :: \<open>[\<lambda>(_, S). length (get_avdom S) \<le> sint64_max]\<^sub>a
+    sint64_nat_assn\<^sup>k *\<^sub>a isasat_bounded_assn\<^sup>d \<rightarrow> isasat_bounded_assn\<close>
+  supply [[goals_limit=1]] length_avdom_def[simp]
+  unfolding mark_clauses_as_unused_wl_D_heur_def
+    mark_unused_st_heur_def[symmetric]
+    access_vdom_at_def[symmetric] length_avdom_def[symmetric]
+  apply (annot_snat_const "TYPE(64)")
+  by sepref
+
+
+sepref_register mark_to_delete_clauses_wl_D_heur
+
+sepref_def mark_to_delete_clauses_wl_D_heur_fast_impl
+  is \<open>mark_to_delete_clauses_wl_D_heur\<close>
+  :: \<open>[\<lambda>S. length (get_clauses_wl_heur S) \<le> sint64_max]\<^sub>a isasat_bounded_assn\<^sup>d \<rightarrow> isasat_bounded_assn\<close>
+  unfolding mark_to_delete_clauses_wl_D_heur_def
+    access_vdom_at_def[symmetric] length_avdom_def[symmetric]
+    get_the_propagation_reason_heur_def[symmetric]
+    clause_is_learned_heur_def[symmetric]
+    clause_lbd_heur_def[symmetric]
+    access_length_heur_def[symmetric]
+    short_circuit_conv mark_to_delete_clauses_wl_D_heur_is_Some_iff
+    marked_as_used_st_def[symmetric] if_conn(4)
+  supply [[goals_limit = 1]] option.splits[split] if_splits[split]
+    length_avdom_def[symmetric, simp] access_vdom_at_def[simp]
+  apply (annot_snat_const "TYPE(64)")
+  apply sepref_dbg_keep
+  apply sepref_dbg_trans_keep
+  apply sepref_dbg_trans_step_keep
+  apply sepref_dbg_side_unfold
+oops
+  by sepref
+
+sepref_register cdcl_twl_full_restart_wl_prog_heur
+
+sepref_def cdcl_twl_full_restart_wl_prog_heur_fast_code
+  is \<open>cdcl_twl_full_restart_wl_prog_heur\<close>
+  :: \<open>[\<lambda>S. length (get_clauses_wl_heur S) \<le> sint64_max]\<^sub>a  isasat_bounded_assn\<^sup>d \<rightarrow> isasat_bounded_assn\<close>
+  unfolding cdcl_twl_full_restart_wl_prog_heur_def
+  supply [[goals_limit = 1]]
+  by sepref
+
+sepref_definition cdcl_twl_restart_wl_heur_code
+  is \<open>cdcl_twl_restart_wl_heur\<close>
+  :: \<open>isasat_unbounded_assn\<^sup>d \<rightarrow>\<^sub>a isasat_unbounded_assn\<close>
+  unfolding cdcl_twl_restart_wl_heur_def
+  supply [[goals_limit = 1]]
+  by sepref
+
+sepref_def cdcl_twl_restart_wl_heur_fast_code
+  is \<open>cdcl_twl_restart_wl_heur\<close>
+  :: \<open>[\<lambda>S. length (get_clauses_wl_heur S) \<le> sint64_max]\<^sub>a isasat_bounded_assn\<^sup>d \<rightarrow> isasat_bounded_assn\<close>
+  unfolding cdcl_twl_restart_wl_heur_def
+  supply [[goals_limit = 1]]
+  by sepref
+
+declare cdcl_twl_restart_wl_heur_fast_code.refine[sepref_fr_rules]
+   cdcl_twl_restart_wl_heur_code.refine[sepref_fr_rules]
+
+
+sepref_def cdcl_twl_full_restart_wl_D_GC_heur_prog_fast_code
+  is \<open>cdcl_twl_full_restart_wl_D_GC_heur_prog\<close>
+  :: \<open>[\<lambda>S. length (get_clauses_wl_heur S) \<le> sint64_max]\<^sub>a isasat_bounded_assn\<^sup>d \<rightarrow> isasat_bounded_assn\<close>
+  unfolding cdcl_twl_full_restart_wl_D_GC_heur_prog_def zero_uint32_nat_def[symmetric]
+  supply [[goals_limit = 1]]
+  by sepref
+
+sepref_register restart_required_heur cdcl_twl_restart_wl_heur
+
+sepref_def restart_prog_wl_D_heur_fast_code
+  is \<open>uncurry2 (restart_prog_wl_D_heur)\<close>
+  :: \<open>[\<lambda>((S, _), _). length (get_clauses_wl_heur S) \<le> sint64_max]\<^sub>a
+      isasat_bounded_assn\<^sup>d *\<^sub>a sint64_nat_assn\<^sup>k *\<^sub>a bool_assn\<^sup>k \<rightarrow> isasat_bounded_assn *a sint64_nat_assn\<close>
+  unfolding restart_prog_wl_D_heur_def
+  supply [[goals_limit = 1]]
+  by sepref
+
+definition isasat_fast_bound where
+  \<open>isasat_fast_bound = uint64_max - (uint32_max div 2 + 6)\<close>
+
+lemma isasat_fast_bound[sepref_fr_rules]:
+   \<open>(uncurry0 (return 18446744071562067962), uncurry0 (RETURN isasat_fast_bound)) \<in>
+   unit_assn\<^sup>k \<rightarrow>\<^sub>a uint64_nat_assn\<close>
+  by sepref_to_hoare (sep_auto simp: uint64_nat_rel_def br_def isasat_fast_bound_def
+     uint64_max_def uint32_max_def)
+
+sepref_register isasat_fast
+sepref_def isasat_fast_code
+  is \<open>RETURN o isasat_fast\<close>
+  :: \<open>isasat_bounded_assn\<^sup>k \<rightarrow>\<^sub>a bool_assn\<close>
+  unfolding isasat_fast_alt_def isasat_bounded_assn_def isasat_fast_bound_def[symmetric]
+  supply [[goals_limit = 1]] uint32_max_nat_hnr[sepref_fr_rules]
+  by sepref
+
+declare isasat_fast_code.refine[sepref_fr_rules]
+
+
+sepref_def cdcl_twl_stgy_restart_prog_wl_heur_fast_code
+  is \<open>cdcl_twl_stgy_restart_prog_early_wl_heur\<close>
+  :: \<open>[\<lambda>S. isasat_fast S]\<^sub>a isasat_bounded_assn\<^sup>d \<rightarrow> isasat_unbounded_assn\<close>
+  unfolding cdcl_twl_stgy_restart_prog_early_wl_heur_def
+  supply [[goals_limit = 1]] isasat_fast_def[simp]
+  by sepref
+
+declare cdcl_twl_stgy_restart_prog_wl_heur_fast_code.refine[sepref_fr_rules]
+
+end
